verified/entry.s.dfy
@@ -5,6 +5,18 @@ include "smcapi.s.dfy"
 include "pagedb.i.dfy"
 include "abstate.s.dfy"
 
+predicate nonStoppedL1(d:PageDb, l1:PageNr)
+{
+    validL1PTPage(d, l1) && (validPageDbImpliesWellFormed(d);
+        !hasStoppedAddrspace(d, l1))
+}
+
+predicate nonStoppedDispatcher(d:PageDb, p:PageNr)
+{
+    validDispatcherPage(d,p) && (validPageDbImpliesWellFormed(d);
+        !hasStoppedAddrspace(d,p))
+}
+
 function l1pOfDispatcher(d:PageDb, p:PageNr) : PageNr
     requires validDispatcherPage(d, p) && !hasStoppedAddrspace(d, p)
     ensures  validL1PTPage(d, l1pOfDispatcher(d, p))
@@ -13,6 +25,7 @@ function l1pOfDispatcher(d:PageDb, p:PageNr) : PageNr
     d[d[p].addrspace].entry.l1ptnr
 }
 
+
 // This must hold between all consecutive states on the addsrpace entry/return path.
 predicate validERTransition(s:SysState, s':SysState)
 {
@@ -20,14 +33,13 @@ predicate validERTransition(s:SysState, s':SysState)
     validSysState(s) && validSysState(s') &&
     (var sd := s.g.g_cur_dispatcher;
     var sd' := s'.g.g_cur_dispatcher;
-    validERTransitionHW(s.hw, s'.hw, s.d) &&
-    s.g.g_cur_dispatcher == s'.g.g_cur_dispatcher &&
-    validDispatcherPage(s.d, sd) && !hasStoppedAddrspace(s.d, sd) &&
-    validL1PTPage(s.d, l1pOfDispatcher(s.d, sd)) && 
-    validDispatcherPage(s'.d, sd') && !hasStoppedAddrspace(s'.d, sd) &&
-    validL1PTPage(s'.d, l1pOfDispatcher(s'.d, sd')) &&
-    l1pOfDispatcher(s.d, s.g.g_cur_dispatcher)  == s.hw.conf.ttbr0 &&
-    l1pOfDispatcher(s'.d, s'.g.g_cur_dispatcher) == s'.hw.conf.ttbr0)
+    validERTransitionHW(s.hw, s'.hw, s.d) && sd == sd'
+    && equivalentExceptPage(s.d, s'.d, sd) 
+    && nonStoppedDispatcher(s.d, sd) && nonStoppedDispatcher(s'.d, sd')
+    && l1pOfDispatcher(s.d, sd)  == s.hw.conf.ttbr0
+    && l1pOfDispatcher(s'.d, sd') == s'.hw.conf.ttbr0
+    && WSMemInvariantExceptAddrspaceAtPage(s.hw, s'.hw, s.d,
+        l1pOfDispatcher(s.d, sd)))
 
 }
 
@@ -37,16 +49,59 @@ predicate validERTransitionHW(hw:state, hw':state, d:PageDb)
     reveal_ValidConfig();
     ValidState(hw) && ValidState(hw')
     && hw'.conf.ttbr0 == hw.conf.ttbr0 
-    && validL1PTPage(d, hw.conf.ttbr0)
-    && validL1PTPage(d, hw'.conf.ttbr0)
-    && !hasStoppedAddrspace(d, hw.conf.ttbr0)
-    && !hasStoppedAddrspace(d, hw'.conf.ttbr0)
+    && nonStoppedL1(d, hw.conf.ttbr0)
+    && bankedRegsPreserved(hw, hw')
 }
 
-predicate validEntryTransitionEnter(s:SysState,s':SysState,
+predicate validSysStates(sset:set<SysState>) { forall s :: s in sset ==> validSysState(s) }
+
+predicate validEnter(s:SysState,s':SysState,
     dispPage:PageNr,a1:int,a2:int,a3:int)
     requires isUInt32(a1) && isUInt32(a2) && isUInt32(a3) && validSysState(s)
     requires smc_enter(s.d, dispPage, a1, a2, a3).1 == KEV_ERR_SUCCESS()
+{
+    reveal_ValidRegState();
+    // smc_enter(s.d, dispPage, a1, a2, a3).1 != KEV_ERR_SUCCESS() ||
+    
+    // s1 (s)  : State on entry to the monitor
+    // s2      : prior to MOVSPCLR that transitions to userspace
+    // s3      : post MOVS State just before start of userspace execution
+    // s4      : Exceptional state where handler must be called
+    // s5      : State at start of exception handler
+    // s6      : State at start of transition back to smc_handler
+    // s7      : State on re-entry to smc_handler
+    // s8 (s') : State at the end of the monitor call/
+    
+    // s4 == s5 except not in exceptional state in s4
+    // s6 == s7 except branch has happened
+    
+    (exists s2, s3, s4 :: validSysStates({s2,s3,s4})
+        && preEntryEnter(s,s2,dispPage,a1,a2,a3)
+        && entryTransitionEnter(s2, s3)
+        && s4.d == s3.d && userspaceExecution(s3.hw, s4.hw, s3.d)
+        && validERTransition(s4, s')
+        && (s'.hw.regs[R0], s'.hw.regs[R1], s'.d) ==
+            exceptionHandled(s4, dispPage)
+        && s'.hw.conf.scr.ns == NotSecure)
+}
+
+/*
+predicate validResume(s:SysState,s':SysState,dispPage:PageNr)
+    requires validSysState(s)
+{
+     
+    smc_resume(s.d, dispPage).1 != KEV_ERR_SUCCESS() ||
+        ... state transitions
+}
+*/
+
+predicate preEntryEnter(s:SysState,s':SysState,
+    dispPage:PageNr,a1:int,a2:int,a3:int)
+    requires isUInt32(a1) && isUInt32(a2) && isUInt32(a3) && validSysState(s)
+    requires smc_enter(s.d, dispPage, a1, a2, a3).1 == KEV_ERR_SUCCESS()
+    ensures  nonStoppedL1(s.d, l1pOfDispatcher(s.d, dispPage));
+    // ensures (validSysState(s) && validSysState(s') && 
+    // preEntryEnter(s,s',dispPage,a1,a2,a3)) ==>false
 {
     reveal_validPageDb();
     reveal_ValidConfig();
@@ -54,7 +109,7 @@ predicate validEntryTransitionEnter(s:SysState,s':SysState,
 	//var addrspace := s.d[s.d[dispPage].addrspace].entry;
     var l1p := l1pOfDispatcher(s.d, dispPage);
     
-    validSysState(s') && s'.d == s.d &&
+    validSysState(s') &&  s.d == s'.d &&
     s'.hw.conf.ttbr0 == l1p &&
     s'.hw.conf.cpsr.m  == User && s'.hw.conf.scr.ns == Secure &&
     
@@ -62,16 +117,13 @@ predicate validEntryTransitionEnter(s:SysState,s':SysState,
 
     s'.g.g_cur_dispatcher == dispPage &&
 
-    bankedRegsPreservedForMonitor(s.hw, s'.hw) &&
-    WSMemInvariantExceptAddrspaceAtPage(s.hw, s'.hw, s.d, l1p) &&
+    bankedRegsPreserved(s.hw, s'.hw) &&
+    WSMemInvariantExceptAddrspaceAtPage(s.hw, s'.hw, s.d, l1p)
 
-    // ENTER_ADDRSPACE is instruction evaluated on s->s'
-    // sp_eval(Ins(MOVS_PCLR), s.hw, s'.hw, true) &&
-    OperandContents(s.hw, OLR) == s.d[dispPage].entry.entrypoint
 }
 
 /*
-predicate validEntryTransitionResume(s:SysState, s':SysState, dispPage:PageNr)
+predicate preEntryResume(s:SysState, s':SysState, dispPage:PageNr)
     requires validSysState(s)
     requires smc_resume(s.d, dispPage).1 == KEV_ERR_SUCCESS()
 {
@@ -104,174 +156,76 @@ predicate validEntryTransitionResume(s:SysState, s':SysState, dispPage:PageNr)
     s'.hw.sregs[cpsr] == disp.ctxt.cpsr &&
     s'.hw.conf.cpsr == decode_psr(disp.ctxt.cpsr)) &&
     
-    bankedRegsPreservedForMonitor(s, s') &&
-    WSMemInvariantExceptAddrspaceAtPage(s.hw, s'.hw, d, l1pOfDispatcher(s.d, dispPage)) &&
+    bankedRegsPreserved(s, s') &&
+    WSMemInvariantExceptAddrspaceAtPage(s.hw, s'.hw, d, l1pOfDispatcher(s.d, dispPage))
 
+}
+*/
+
+predicate entryTransitionEnter(s:SysState,s':SysState)
+    // ensures (validSysState(s) && validSysState(s') && entryTransitionEnter(s,s')) ==>false
+{
+    validERTransition(s, s') && s'.d == s.d &&
     sp_eval(Ins(MOVS_PCLR), s.hw, s'.hw, true) &&
-    OperandContents(s.hw, OLR) == disp.ctxt.pc
+    OperandContents(s.hw, OLR) == s.d[s.g.g_cur_dispatcher].entry.entrypoint
 }
-*/
 
-predicate eqDisp(s:SysState, s':SysState) { s.g.g_cur_dispatcher == s'.g.g_cur_dispatcher }
-
-predicate validEnter(s:SysState,s':SysState,
-    dispPage:PageNr,a1:int,a2:int,a3:int)
-    requires isUInt32(a1) && isUInt32(a2) && isUInt32(a3) && validSysState(s)
+predicate entryTransitionResume(s:SysState,s':SysState)
+    // ensures (validSysState(s) && validSysState(s') && entryTransitionResume(s,s')) ==>false
 {
-    // s0 (s)  : State on entry to the monitor
-    // s1      : prior to MOVSPCLR that transitions to userspace/a
-    // s2      : post MOVS State just before start of userspace execution.
-    // s3      : Exceptional where handler must be called
-    // s4      : State at start of exception handler
-    // s5      : State at start of transition back to smc_handler
-    // s6      : State on re-entry to smc_handler
-    // s7 (s') : State at the end of the monitor call/
-    //
-    // s3 == s4 except not in exceptional state in s4
-    // s5 == s6 except branch has happened
-    
-    smc_enter(s.d, dispPage, a1, a2, a3).1 != KEV_ERR_SUCCESS() ||
-    (exists s2, s3, s4, s5 :: validSysState(s2) && validSysState(s3)
-        && validSysState(s4) && validSysState(s5)
-        && validEntryTransitionEnter(s,s2,dispPage,a1,a2,a3)
-        && s3.d == s2.d && userspaceExecution(s2.hw, s3.hw, s2.d)
-        && s4.d == s3.d && handlerCalled(s3.hw, s4.hw)
-        && exceptionHandled(s4, s5)
-        && monitorReturn(s5, s'))
+    validSysState(s) && validSysState(s') && s.d == s'.d &&    
+    (var disp := s.d[s.g.g_cur_dispatcher].entry;
+    sp_eval(Ins(MOVS_PCLR), s.hw, s'.hw, true) &&
+    OperandContents(s.hw, OLR) == disp.ctxt.pc)
 }
 
-/*
-predicate validResume(s:SysState,s':SysState,dispPage:PageNr)
+predicate userspaceExecution(hw:state, hw':state, d:PageDb)
+    /*ensures (exists s, s' :: validSysState(s) && validSysState(s') &&
+        s.d == s'.d && userspaceExecution(s.hw, s'.hw, d)) ==> false */
+{
+    validERTransitionHW(hw, hw', d)
+    && hw.conf.cpsr.m == User && hw'.conf.cpsr.m == User
+    && WSMemInvariantExceptAddrspace(hw, hw', d)
+    && !hw'.conf.ex.none?
+}
+
+//-----------------------------------------------------------------------------
+// Exception Handler Spec
+//-----------------------------------------------------------------------------
+function exceptionHandled(s:SysState,p:PageNr) : (int, int, PageDb)
     requires validSysState(s)
+    requires !s.hw.conf.ex.none?
 {
-    // s1 (s)  : State on entry to the monitor
-    // s2      : State just before start of userspace execution.
-    // s3      : State between end of userspace execution and the exception handler
-    // s4      : State between the exception handler and re-entry to the monitor
-    // s5 (s') : State at the end of the monitor call
-     
-    smc_resume(s.d, dispPage).1 != KEV_ERR_SUCCESS() ||
-    (exists s2, s3, s4 :: validEntryTransitionResume(s,s2,dispPage) 
-        && userspaceExecution(s2, s3)
-        && exceptionHandled(s3, s4)
-        && monitorReturn(s4, s'))
-}
-*/
-
-predicate exceptionHandled(s:SysState,s':SysState)
-    ensures exceptionHandled(s, s') ==> 
-        validERTransition(s, s') &&
-        WSMemInvariantExceptAddrspace(s.hw, s'.hw, s.d)
-{
-    svc(s,s') || irqfiq(s,s') || abort(s,s')
-}
-
-predicate handlerCalled(hw:state,hw':state)
-{
-    !hw.conf.ex.none? &&
-    ValidState(hw) &&
-    hw'  == hw.(conf := hw.conf.(ex := none))
-}
-
-predicate monitorReturn(s:SysState,s':SysState)
-{
-    reveal_ValidRegState();
-    validERTransition(s, s')
-    && s'.d == s.d
-    && WSMemInvariantExceptAddrspace(s.hw, s'.hw, s.d)
-    && bankedRegsPreservedForMonitor(s.hw, s'.hw)
-    && s'.hw.conf.scr.ns == NotSecure
-}
-
-predicate svc(s:SysState,s':SysState) 
-{
-    reveal_ValidRegState();
-    
-    validERTransition(s, s') &&
-    s.hw.conf.cpsr.m == Supervisor &&
-    s'.hw.conf.cpsr.m == Monitor &&
-    s.hw.conf.ex.svc? &&
-    
-    WSMemInvariantExceptAddrspace(s.hw, s'.hw, s.d) &&
-    bankedRegsPreservedForMonitor(s.hw, s'.hw) &&
-    
-    s'.hw.regs[R0] == KEV_ERR_SUCCESS()  &&
-        
-    s'.d == s.d
-}
-
-predicate irqfiq(s:SysState,s':SysState)
-{
-    reveal_ValidRegState();
+    reveal_validPageDb();
     reveal_ValidSRegState();
-    reveal_ValidConfig();
-    
-    validERTransition(s, s') &&
-    s.hw.conf.cpsr.m == Monitor &&
-    s'.hw.conf.cpsr.m == Monitor &&
-    (s.hw.conf.ex.irq? || s.hw.conf.ex.fiq?) &&
-
-    WSMemInvariantExceptAddrspace(s.hw, s'.hw, s.d) &&
-    bankedRegsPreservedForMonitor(s.hw, s'.hw) &&
-    
-    // Interrupts can be taken from other modes, but the interrupt should
-    // only re-enter monitor mode when taken from user mode. The following 
-    // condition checks that this interrupt was taken from user mode.
-    s.hw.conf.spsr[Monitor].m == User &&
-
-    s'.hw.regs[R0] == KEV_ERR_INTERRUPTED() &&
-    
-    (var dispPage := s.g.g_cur_dispatcher;
-    validDispatcherPage(s'.d, dispPage) &&
-    s'.d[dispPage].addrspace == s.d[dispPage].addrspace &&
-    s'.d[dispPage].entry.entered == true &&
-    s'.d[dispPage].entry.ctxt.regs == s.hw.regs &&
-    s'.d[dispPage].entry.ctxt.pc == OperandContents(s.hw, OLR) &&
-    s'.d[dispPage].entry.ctxt.cpsr == s.hw.sregs[cpsr] &&
-    equivalentExceptPage(s.d, s'.d, dispPage))
-
-}
-
-predicate abort(s:SysState,s':SysState)
-{
     reveal_ValidRegState();
-   
-    validERTransition(s, s') &&
-    s.hw.conf.cpsr.m == Abort  &&
-    s'.hw.conf.cpsr.m == Monitor &&
-    s.hw.conf.ex.abt? &&
-    
-    s.d == s'.d &&
-    bankedRegsPreservedForMonitor(s.hw, s'.hw) &&
-    WSMemInvariantExceptAddrspace(s.hw, s'.hw, s.d) &&
-
-    s'.hw.regs[R0] == KEV_ERR_FAULT() &&
-    
-    (var dispPage := s.g.g_cur_dispatcher;
-    validDispatcherPage(s'.d, dispPage) &&
-    s'.d[dispPage].addrspace == s.d[dispPage].addrspace &&
-    s'.d[dispPage].entry.entered == true)
+    reveal_ValidConfig();
+    if(s.hw.conf.ex.svc?) then (KEV_ERR_SUCCESS(), 0, s.d)
+    else 
+        var p := s.g.g_cur_dispatcher;
+        var pc := OperandContents(s.hw, OLR);
+        var cpsr := s.hw.sregs[cpsr];
+        var disp' := Dispatcher(s.d[p].entry.entrypoint, true,
+            DispatcherContext(s.hw.regs, cpsr, pc));
+        var d' := s.d[ p := PageDbEntryTyped(s.d[p].addrspace, disp')];
+        if(s.hw.conf.ex.irq? || s.hw.conf.ex.fiq?) then
+            (KEV_ERR_INTERRUPTED(), 0, d')
+        else
+            assert s.hw.conf.ex.abt?;
+            (KEV_ERR_FAULT(), 0, d')
 }
 
 //-----------------------------------------------------------------------------
 // Userspace Execution
 //-----------------------------------------------------------------------------
 
-predicate userspaceExecution(hw:state, hw':state, d:PageDb)
-{
-    validERTransitionHW(hw, hw', d)
-    && hw.conf.cpsr.m == User && hw'.conf.cpsr.m == User
-    && WSMemInvariantExceptAddrspace(hw, hw', d)
-    && bankedRegsPreservedForMonitor(hw, hw')
-    && !hw'.conf.ex.none?
-}
 
-predicate bankedRegsPreservedForMonitor(hw:state, hw':state)
+predicate bankedRegsPreserved(hw:state, hw':state)
     requires ValidState(hw) && ValidState(hw')
 {
         reveal_ValidRegState();
         reveal_ValidConfig();
-        var m := Monitor;
+        forall m :: m != User ==>
         hw.conf.spsr[m] == hw'.conf.spsr[m] &&
         hw.regs[LR(m)] == hw'.regs[LR(m)] &&
         hw.regs[SP(m)] == hw'.regs[SP(m)]
@@ -289,15 +243,13 @@ predicate WSMemInvariantExceptAddrspace(hw:state, hw':state, d:PageDb)
 
 predicate WSMemInvariantExceptAddrspaceAtPage(hw:state, hw':state, 
         d:PageDb, l1p:PageNr)
-    requires ValidState(hw) && ValidState(hw')
-    requires validL1PTPage(d, l1p)
-    requires (validPageDbImpliesWellFormed(d); !hasStoppedAddrspace(d, l1p))
+    requires ValidState(hw) && ValidState(hw') && nonStoppedL1(d, l1p)
 {
     (forall m:mem :: m in hw.m.addresses <==> m in hw'.m.addresses) &&
     hw.m.globals == hw'.m.globals &&
-    forall i :: i in hw.m.addresses && address_is_secure(i) &&
-        !memSWrInAddrspace(d, l1p, i) ==>
-            hw.m.addresses[i] == hw'.m.addresses[i]
+    (forall i | i in hw.m.addresses && address_is_secure(i) && 
+        !memSWrInAddrspace(d, l1p, i) ::  
+            hw.m.addresses[i] == hw'.m.addresses[i])
 }
 
 
@@ -317,7 +269,7 @@ predicate memSWrInAddrspace(d:PageDb, l1p:PageNr, m: mem)
     requires validL1PTPage(d, l1p)
     requires (validPageDbImpliesWellFormed(d); !hasStoppedAddrspace(d, l1p))
 {
-    exists p :: validPageNr(p) && pageSWrInAddrspace(d, l1p, p) && addrInPage(m, p)
+    exists p | validPageNr(p) :: pageSWrInAddrspace(d, l1p, p) && addrInPage(m, p)
 }
 
 // is the page secure, writeable, and in the L2PT
@@ -329,48 +281,11 @@ predicate pageSWrInL2PT(l2pt:seq<L2PTE>, p:PageNr)
         case InsecureMapping(p',w) => false)
 }
 
-
-
-// A purely abstract version of the memory invariant
 predicate equivalentExceptPage(d:PageDb, d':PageDb, p:PageNr)
     requires validPageNr(p)
     requires validPageDb(d) && validPageDb(d')
 {
     validPageDbImpliesWellFormed(d);
     validPageDbImpliesWellFormed(d');
-    forall p' :: validPageNr(p') && p' != p ==> d[p'] == d'[p]
+    forall p' :: validPageNr(p') && p' != p ==> d[p'] == d'[p']
 }
-
-
-// Copied from old entry.s.dfy
-// //-----------------------------------------------------------------------------
-// // Safety poperties of the monitor/addrspace boundary
-// //-----------------------------------------------------------------------------
-// 
-// predicate addrspaceOwnershipOfPagesPreserved(d:PageDb, d':PageDb)
-//     // requires userEnteredState(s, d) && userEnteredState(s', d')
-//     requires validPageDb(d) && validPageDb(d')
-// {
-//     reveal_validPageDb();
-//     forall a :: validAddrspacePage(d, a) ==>
-//         validAddrspacePage(d', a) && 
-//         (var l1 := d[a].entry.l1ptnr;
-//         forall m :: !hasStoppedAddrspace(d,a) && memSWrInAddrspace(d, l1, m) ==> 
-//             d'[a] == d[a] && !hasStoppedAddrspace(d', a) && memSWrInAddrspace(d', l1, m))
-// }
-// 
-// // The pages owned by other addrspaces are preserved
-// predicate addrspaceContentsPreservedExcept(s:state, s':state, d: PageDb, d':PageDb, disp:PageNr)
-//     requires userEnteredState(s, d) && userEnteredState(s', d')
-//     requires addrspaceOwnershipOfPagesPreserved(d, d')
-//     requires valid
-// {
-//     reveal_validPageDb();
-//     var a := d[disp].addrspace;
-//     ValidState(s') && AlwaysInvariant(s, s') &&
-//     forall a' :: validAddrspacePage(d, a') && a' != a && 
-//       !hasStoppedAddrspace(d, a') ==>
-//         (var l1' := d[a'].entry.l1ptnr;
-//         forall m :: memSWrInAddrspace(d, l1', m) ==>
-//             s.m.addresses[m] == s'.m.addresses[m])
-// }
